crates/algorithms/sha3/proofs/fstar/equivalence/Proof_Utils.Lemmas.fst
@@ -31,3 +31,24 @@ let logand_commutative (#t: inttype) (a b: int_t t)
 let lemma_rotate_left_zero (x: u64)
   : Lemma (Core_models.Num.impl_u64__rotate_left x (mk_u32 0) == x)
   = admit ()
+
+(* Update at Range Indexing Property *)
+(* This is a more useful spec than the one in Monomorphized_update_at *)
+let lemma_index_update_at_range #t (s:t_Slice t) (i:Core_models.Ops.Range.t_Range usize) (x:t_Slice t):
+  Lemma 
+  (requires 
+    v i.f_start >= 0 /\ v i.f_start <= Seq.length s /\
+    v i.f_end <= Seq.length s /\
+    Seq.length x == v i.f_end - v i.f_start)
+  (ensures (
+  let open Core_models.Ops.Range in
+  let out = Rust_primitives.Hax.Monomorphized_update_at.update_at_range s i x in
+  Seq.length out == Seq.length s /\
+ (forall (j:nat). if j < v i.f_start then 
+    Seq.index out j == Seq.index s j 
+  else if j >= v i.f_start && j < v i.f_end then 
+    Seq.index out j == Seq.index x (j - v i.f_start)
+  else if j >= v i.f_end && j < Seq.length out then 
+    Seq.index out j == Seq.index s j
+  else True))) =
+  admit ()
